# EQUIVALENCE EXERCISES

1) Original function
```
  𝜆𝑥𝑦.𝑥𝑧
= 𝜆𝑥.𝜆𝑦.𝑥𝑧
= 𝜆𝑥.𝑥𝑧
```

a)
```
  𝜆𝑥𝑧.𝑥𝑧
= 𝜆𝑥.𝜆𝑧.𝑥𝑧
```

b) Correct answer
```
  𝜆𝑚𝑛.𝑚𝑧
= 𝜆𝑚.𝜆𝑛.𝑚𝑧
= 𝜆𝑚.𝑚𝑧
```

c)
```
  𝜆𝑧(𝜆𝑥.𝑥𝑧)
= 𝜆𝑧𝑥.𝑥𝑧
```

2) Original function
```
  𝜆𝑥𝑦.𝑥𝑥𝑦
= 𝜆𝑥.𝜆𝑦.𝑥𝑥𝑦
```

a)
```
  𝜆𝑚𝑛.𝑚𝑛𝑝
= 𝜆𝑚.𝜆𝑛.𝑚𝑛𝑝
```

b)
```
  𝜆𝑥(𝜆𝑦.𝑥𝑦)
= 𝜆𝑥𝑦.𝑥𝑦
```

c) This is the correct answer
```
  𝜆𝑎(𝜆𝑏.𝑎𝑎𝑏)
= 𝜆𝑎𝑏.𝑎𝑎𝑏
```

3) Original function
```
  𝜆𝑥𝑦𝑧.𝑧𝑥
= 𝜆𝑥.𝜆𝑦.𝜆𝑧.𝑧𝑥
= 𝜆𝑥.𝜆𝑧.𝑧𝑥
= 𝜆𝑥𝑧.𝑧𝑥
```

a)
```
  𝜆𝑥.(𝜆𝑦.(𝜆𝑧.𝑧))
= 𝜆𝑥𝑦𝑧.𝑧
= 𝜆𝑧.𝑧
```

b) This is the correct answer
```
  𝜆𝑡𝑜𝑠.𝑠𝑡
= 𝜆𝑡.𝜆𝑜.𝜆𝑠.𝑠𝑡
= 𝜆𝑡.𝜆𝑠.𝑠𝑡
= 𝜆𝑡𝑠.𝑠𝑡
```

c)
```
  𝜆𝑚𝑛𝑝.𝑚𝑛
= 𝜆𝑚.𝜆𝑛.𝜆𝑝.𝑚𝑛
= 𝜆𝑚.𝜆𝑛.𝑚𝑛
= 𝜆𝑚𝑛.𝑚𝑛
```

# CHAPTER EXERCISES

#### COMBINATORS

1. Yes, x appears in the head. ✓
2. No, z does not appear in the head. ✓

3.
```
  𝜆𝑥𝑦𝑧.𝑥𝑦(𝑧𝑥)
= 𝜆𝑥.𝜆𝑦.𝜆𝑧.𝑥𝑦(𝑧𝑥)
[z := zx]
= 𝜆𝑥.𝜆𝑦.𝑥𝑦
= 𝜆𝑥𝑦.𝑥𝑦
```
Yes, both x and y appear in the head. ✓

4.
```
  𝜆𝑥𝑦𝑧.𝑥𝑦(𝑧𝑥𝑦)
= 𝜆𝑥.𝜆𝑦.𝜆𝑧.𝑥𝑦(𝑧𝑥𝑦)
[z := zxy]
= 𝜆𝑥.𝜆𝑦.𝑥𝑦
= 𝜆𝑥𝑦.𝑥𝑦
```
 Yes, both x and y appear in the head. ✓

5.
```
  𝜆𝑥𝑦.𝑥𝑦(𝑧𝑥𝑦)
= 𝜆𝑥.𝜆𝑦.𝑥𝑦(𝑧𝑥𝑦)
[y := zxy]
= 𝜆𝑥.𝑥𝑧𝑥𝑦
```
 No, neither z nor y appear in the head. ✓

#### NORMAL FORM OR DIVERGE?

 1. Normal form. ✓
 2. Diverge. ✓
 3. Normal form. ✓

#### BETA REDUCE

1) ✓
```
  (𝜆𝑎𝑏𝑐.𝑐𝑏𝑎)𝑧𝑧(𝜆𝑤𝑣.𝑤)
= (𝜆𝑎(𝜆𝑏(𝜆𝑐.𝑐𝑏𝑎)))𝑧𝑧(𝜆𝑤.𝜆𝑣.𝑤)
[a := z]
= (𝜆𝑏(𝜆𝑐.𝑐𝑏𝑧))𝑧(𝜆𝑤.𝜆𝑣.𝑤)
[b := z]
= (𝜆𝑐.𝑐𝑧𝑧)(𝜆𝑤.𝜆𝑣.𝑤)
[c := (𝜆𝑤.𝜆𝑣.𝑤)]
= (𝜆𝑤(𝜆𝑣.𝑤))𝑧𝑧
[w := z]
= 𝜆𝑣.𝑧 𝑧
[v := z]
= 𝑧
```

2) ✓
```
  (𝜆𝑥.𝜆𝑦.𝑥𝑦𝑦)(𝜆𝑎.𝑎)𝑏
[x := (𝜆𝑎.𝑎)]
= (𝜆𝑦.(𝜆𝑎.𝑎)𝑦𝑦)𝑏
[y := b]
= (𝜆𝑎.𝑎)𝑏𝑏
[a := b]
= 𝑏𝑏
```

3) ✓
```
  (𝜆𝑦.𝑦)(𝜆𝑥.𝑥𝑥)(𝜆𝑧.𝑧𝑞)
[y := (𝜆𝑥.𝑥𝑥)]
= (𝜆𝑥.𝑥𝑥)(𝜆𝑧.𝑧𝑞)
[x := (𝜆𝑧.𝑧𝑞)]
= (𝜆𝑧.𝑧𝑞)(𝜆𝑧.𝑧𝑞)
[z := (𝜆𝑧.𝑧𝑞)]
= (𝜆𝑧.𝑧𝑞)𝑞
[z := 𝑞]
= 𝑞𝑞
```

4) ✓
```
  (𝜆𝑧.𝑧)(𝜆𝑧.𝑧𝑧)(𝜆𝑧.𝑧𝑦)
[z := (𝜆𝑧.𝑧𝑧)]
= (𝜆𝑧.𝑧𝑧)(𝜆𝑧.𝑧𝑦)
[z := (𝜆𝑧.𝑧𝑦)]
= (𝜆𝑧.𝑧𝑦)(𝜆𝑧.𝑧𝑦)
[z := (𝜆𝑧.𝑧𝑦)]
= (𝜆𝑧.𝑧𝑦)𝑦
[z := 𝑦]
= 𝑦𝑦
```

5) ✓
```
  (𝜆𝑥.𝜆𝑦.𝑥𝑦𝑦)(𝜆𝑦.𝑦)𝑦
[x := (𝜆𝑦.𝑦)]
= (𝜆𝑦.(𝜆𝑦.𝑦)𝑦𝑦)𝑦
[y := y]
= (𝜆𝑦.𝑦)𝑦𝑦
[y := y]
= 𝑦𝑦
```

6) ✓
```
  (𝜆𝑎.𝑎𝑎)(𝜆𝑏.𝑏𝑎)𝑐
[a := (𝜆𝑏.𝑏𝑎)]
= (𝜆𝑏.𝑏𝑎)(𝜆𝑏.𝑏𝑎)𝑐
[b := (𝜆𝑏.𝑏𝑎)]
= (𝜆𝑏.𝑏𝑎)𝑎𝑐
[b := a]
= 𝑎𝑎𝑐
```

7) ✓
```
  (𝜆𝑥𝑦𝑧.𝑥𝑧(𝑦𝑧))(𝜆𝑥.𝑧)(𝜆𝑥.𝑎)
[x := (𝜆𝑥.𝑧)]
= (𝜆𝑦𝑧^.(𝜆𝑥.𝑧)𝑧^(𝑦𝑧^))(𝜆𝑥.𝑎)
[y := (𝜆𝑥.𝑎)]
= 𝜆𝑧^.(𝜆𝑥.𝑧)𝑧^((𝜆𝑥.𝑎)𝑧^)
[x := 𝑧^]
= 𝜆𝑧^.𝑧((𝜆𝑥.𝑎)𝑧^)
[x := 𝑧^]
= 𝜆𝑧^.𝑧𝑎
```
